theories/Sat.v
@@ -79,10 +79,15 @@ Fixpoint search (σ: Map.map term) E: list term :=
       [v_fanout v0 v1]
 
   | E_app E E' =>
-      do tuple <- search σ E ;
       do v0 <- search σ E' ;
-      do ab <- (if tuple is v_fanout a b then [(a, b)] else []) ;
-      if eq_term v0 (fst ab) then [snd ab] else []
+      do tuple <- search σ E ;
+      if tuple is v_fanout a b
+      then
+        if eq_term v0 a
+        then [b]
+        else []
+      else
+        []
 
   | E_tt => [v_tt]
   | E_step E E' =>
@@ -100,8 +105,36 @@ Fixpoint search (σ: Map.map term) E: list term :=
       search (Map.add x (fst ab) (Map.add y (snd ab) σ)) E'
   end%list.
 
+Lemma Forall_concat:
+  forall {A} p (x: list (list A)), List.Forall (List.Forall p) x -> List.Forall p (List.concat x).
+Proof.
+  all: intros.
+  induction H.
+  1: econstructor.
+  cbn.
+  induction H.
+  1: auto.
+  cbn.
+  econstructor.
+  1: auto.
+  auto.
+Qed.
+
+Theorem Forall_flat_map:
+  forall {A B} p (f: A -> list B) x, List.Forall (fun x => List.Forall p (f x)) x -> List.Forall p (List.flat_map f x).
+Proof.
+  intros.
+  rewrite List.flat_map_concat_map.
+  apply Forall_concat.
+  induction H.
+  1:econstructor.
+  econstructor.
+  1: auto.
+  auto.
+Qed.
+
 Theorem search_sound:
-  forall σ E v, List.In v (search σ E) -> sat σ E v.
+  forall σ E, List.Forall (sat σ E) (search σ E).
 Proof.
   intros σ E.
   generalize dependent σ.
@@ -109,21 +142,81 @@ Proof.
   all: cbn.
   all: intros.
   all: try contradiction.
-  - econstructor.
-    destruct (Map.find x σ).
-    2: inversion H.
-    inversion H.
-    2: inversion H0.
-    subst.
-    auto.
-  - admit.
-  - admit.
-  - destruct H.
-    2: contradiction.
-    subst.
+  - destruct (Map.find x σ) eqn:q.
+    2: econstructor.
     econstructor.
-  - admit.
-  - admit.
+    2:  econstructor.
+    econstructor.
+    auto.
+  - apply Forall_flat_map.
+    induction (generate t).
+    1: econstructor.
+    econstructor.
+    2: auto.
+    apply Forall_flat_map.
+    induction (IHE (Map.add x a σ)).
+    1: econstructor.
+    econstructor.
+    2: auto.
+    econstructor.
+    2: econstructor.
+    econstructor.
+    apply H.
+  - apply Forall_flat_map.
+    induction (IHE2 σ).
+    1: econstructor.
+    econstructor.
+    2: auto.
+    apply Forall_flat_map.
+    induction (IHE1 σ).
+    1: econstructor.
+    cbn.
+    econstructor.
+    destruct x0.
+    all: try econstructor.
+    destruct (eq_term x x0_1).
+    2: constructor.
+    all: cbn.
+    2: apply IHf0.
+    2: auto.
+    1: subst.
+    1: constructor.
+    1: econstructor.
+    1: eauto.
+    1: auto.
+    1: econstructor.
+    admit.
+  - all: repeat constructor.
+  - apply Forall_flat_map.
+    induction (IHE1 σ).
+    1: constructor.
+    constructor.
+    2: apply IHf.
+    destruct x.
+    all: cbn.
+    all: try constructor.
+    rewrite List.app_nil_r.
+    induction (IHE2 σ).
+    1: constructor.
+    constructor.
+    + constructor.
+      all: auto.
+    + admit.
+  - apply Forall_flat_map.
+    induction (IHE1 σ).
+    1: constructor.
+    constructor.
+    2: auto.
+    apply Forall_flat_map.
+    induction (IHE2 σ).
+    1: constructor.
+    constructor.
+    2: apply IHf0.
+    + constructor.
+      2: constructor.
+      constructor.
+      all: auto.
+    + admit.
   - admit.
 Admitted.
 
