theories/SpecNotations.v
@@ -5,7 +5,7 @@ Infix "*" := t_prod.
 Notation "Γ ⊢ E 'in' t" := (JE Γ E t) (at level 90).
 Notation "⊢ v 'in' t" := (Jv v t) (at level 90).
 
-Notation "v0 ~> v1" := (step_v v0 v1) (at level 90).
-Notation "v0 *~> v1" := (multi_v v0 v1) (at level 90).
+Notation "v0 ~> v1" := (step v0 v1) (at level 90).
+Notation "v0 *~> v1" := (multi v0 v1) (at level 90).
 
 Notation "Δ ⊢ E [ v ]" := (sat Δ E v) (at level 90).
